work on differentiation rules for Function.foldl and Function.reduce

SciLean/Core/Function.lean
@@ -1,6 +1,9 @@
 import SciLean.Core.FunctionTransformations
+import SciLean.Core.Monads
 import SciLean.Data.Function
 import SciLean.Data.DataArray 
+import SciLean.Core.FloatAsReal
+import SciLean.Tactic.LetEnter
 
 open SciLean
 
@@ -9,22 +12,13 @@ set_option linter.unusedVariables false
 variable 
   {α β ι : Type _}
 
+--------------------------------------------------------------------------------
+-- Function.foldl --------------------------------------------------------------
+--------------------------------------------------------------------------------
+
 section OnEnumType 
 
 variable [EnumType ι] 
-
-/-- Reverse derivative of `Function.foldl` w.r.t. `f` and `init`. It is implemented using `Array`.
-
-  TODO: 
-    1. needs beter implementation but that requires refining EnumType and Index
-    2. add a version with DataArray
--/
-def Function.foldl.fwdDeriv [Add α] [Add β]
-  (f df : ι → α) (dop : β → α → β → α → β×β) (init dinit : β) : β × β := Id.run do
-  let mut bdb := (init,dinit)
-  for i in fullRange ι do
-    bdb := dop bdb.1 (f i) bdb.2 (df i)
-  bdb
 
 variable
   {K : Type _} [IsROrC K]
@@ -48,13 +42,11 @@ theorem Function.foldl.arg_finit.fwdCDeriv_rule
     fun w dw => 
       let fdf := fwdCDeriv K f w dw
       let initdinit := fwdCDeriv K init w dw
-      let dop := fun y x dy dx => fwdCDeriv K (fun (y,x) => op y x) (y,x) (dy,dx)
-      Function.foldl.fwdDeriv fdf.1 fdf.2 dop initdinit.1 initdinit.2
+      let dop := fun (y,dy) (x,dx) => fwdCDeriv K (fun (y,x) => op y x) (y,x) (dy,dx)
+      Function.foldl (fun i => (fdf.1 i, fdf.2 i)) dop initdinit
       := by sorry_proof
 
-
 end OnEnumType 
-
 
 section OnIndexType
 
@@ -115,8 +107,40 @@ def Function.foldl.revDeriv_dataArrayImpl [Add α] [Add β] [PlainDataType α] [
        let (db',da) := dop bj aj db
        das := das.push da
        db := db'
-     das := das.reverse
+       das := das.reverse
      (⟨das, sorry_proof⟩, db))
+
+/-- Reverse derivative of `Function.foldl` w.r.t. `f` and `init`. It is implemented using `Array`.
+
+  TODO: 
+    1. needs beter implementation but that requires refining EnumType and Index
+    2. add a version with DataArray
+-/
+def Function.foldl.revDeriv_dataArrayImpl_alt [Add α] [Add β] [PlainDataType α] [PlainDataType β]
+  (f : ι → α) (op : β → α → β) (dop : β → α → β → β×α) (init : β) : β × (β → DataArrayN α ι×β) := Id.run do
+  let n := Index.size ι
+  let bbs := Function.foldl f (fun (b,bs) a => (op b a, bs.push b)) (init, DataArray.mkEmpty n)
+  let b := bbs.1
+  let bs := bbs.2
+  (b, 
+   fun db => Id.run do
+     let dbdas := Function.foldl 
+       (fun i : Idx n => 
+         let j : Idx n := ⟨n-i.1-1, sorry_proof⟩
+         (f (fromIdx j), bs.get ⟨j.1, sorry_proof⟩))
+       (fun (db,das) (aj,bj) => 
+         let (db', da) := dop bj aj db
+         (db', das.push da))
+       (db, DataArray.mkEmpty n)
+     let db := dbdas.1
+     let das := dbdas.2
+     let das := das.reverse
+     (⟨das, sorry_proof⟩, db))
+
+
+#eval Function.foldl.revDeriv_arrayImpl (fun i : Idx 3 => (i.toFloat + 5)) (fun x y => x * y) (fun x y dxy => (y*dxy, x*dxy)) 1 |>.snd 1
+#eval Function.foldl.revDeriv_dataArrayImpl (fun i : Idx 3 => (i.toFloat + 5)) (fun x y => x * y) (fun x y dxy => (y*dxy, x*dxy)) 1 |>.snd 1
+#eval Function.foldl.revDeriv_dataArrayImpl_alt (fun i : Idx 3 => (i.toFloat + 5)) (fun x y => x * y) (fun x y dxy => (y*dxy, x*dxy)) 1 |>.snd 1
 
 
 variable
@@ -155,3 +179,304 @@ theorem Function.foldl.arg_finit.revCDeriv_rule [PlainDataType X] [PlainDataType
 end OnIndexType
 
 
+
+--------------------------------------------------------------------------------
+-- Function.reduceD ------------------------------------------------------------
+--------------------------------------------------------------------------------
+
+
+section OnVec
+variable
+  [Index ι]
+  {K : Type _} [IsROrC K]
+  {X : Type _} [Vec K X]
+  {Y : Type _} [Vec K Y]
+  {Z : Type _} [Vec K Z]
+  {W : Type _} [Vec K W]
+
+@[fprop]
+theorem Function.reduceD.arg_fdefault.IsDifferentiable_rule
+  (f : W → ι → X) (op : X → X → X) (default : W → X)
+  (hf : IsDifferentiable K f) (hop : IsDifferentiable K (fun (x,y) => op x y)) (hdefault : IsDifferentiable K default)
+  : IsDifferentiable K (fun w => Function.reduceD (f w) op (default w)) := by sorry_proof
+
+@[ftrans]
+theorem Function.reduceD.arg_fdefault.fwdCDeriv_rule
+  (f : W → ι → X) (op : X → X → X) (default : W → X)
+  (hf : IsDifferentiable K f) (hop : IsDifferentiable K (fun (x,y) => op x y)) (hdefault : IsDifferentiable K default)
+  : fwdCDeriv K (fun w => Function.reduceD (f w) op (default w))
+    =
+    fun w dw => 
+      let fdf := fwdCDeriv K f w dw
+      let defaultddefault := fwdCDeriv K default w dw
+      let dop := fun (x,dy) (y,dy) => fwdCDeriv K (fun (x,y) => op x y) (x,y) (dx,dy)
+      Function.reduceD (fun i => (fdf.1 i, fdf.2 i)) dop defaultddefault
+      := by sorry_proof
+
+end OnVec
+
+section OnSemiInnerProductSpace
+
+variable
+  [Index ι]
+  {K : Type _} [IsROrC K]
+  {X : Type _} [SemiInnerProductSpace K X]
+  {Y : Type _} [SemiInnerProductSpace K Y]
+  {Z : Type _} [SemiInnerProductSpace K Z]
+  {W : Type _} [SemiInnerProductSpace K W]
+
+
+/--
+  -- WARNING: `dx'` and `dw` behave differently
+     - `df'` computes gradient in `dx'` 
+     - `df'` computes update to gradient in `dw` 
+  
+  The value of `df'` should be:
+    df' = fun w i x dx' dw => 
+      ((∇ (x':=x;dx'), f w i x'), (dw + ∇ (w':=w;dx'), f w' i x))
+-/
+def ForIn.arg_bf.revDeriv_dataArrayImpl [Index ι] [PlainDataType X] [PlainDataType W] [Zero X] [Zero W]
+  (init : X) (f : W → ι → X → X) (df' : W → ι → X → X → W → X×W) (w : W)
+  : X×(X→X×W) :=
+  let n := Index.size ι
+  if n = 0 then
+    (init, fun _ => 0)
+  else Id.run do
+    -- forward pass
+    let mut xs : DataArray X := .mkEmpty n
+    let mut x := init
+    for i in fullRange ι do
+      xs := xs.push x
+      x := f w i x
+    (x, fun dx' => Id.run do
+      -- backward pass
+      -- TODO: implemente reverse ranges!
+      let mut dx' := dx'
+      let mut dw : W := 0
+      for i in [0:n.toNat] do
+        let j' : Idx n := ⟨n-i.toUSize-1,sorry_proof⟩
+        let j : ι := fromIdx j'
+        let xj := xs.get ⟨j'.1, sorry_proof⟩
+        let (dx'',dw') := df' w j xj dx' dw
+        dx' := dx''
+        dw := dw'
+      (dx',dw))
+
+
+@[ftrans]
+theorem ForIn.forIn.arg_bf.revDerivM_rule' [Index ι] [PlainDataType X] [PlainDataType W]
+  (init : W → X) (f : W → ι → X → X)
+  (hinit : HasAdjDiff K init) (hf : ∀ i, HasAdjDiff K (fun (w,x) => f w i x))
+  : revCDeriv K (fun w => forIn (m:=Id) (fullRange ι) (init w) (fun i y => do pure PUnit.unit; pure <| ForInStep.yield (f w i y))) 
+    =
+    fun w => 
+      let initdinit := revCDeriv K init w
+      let forInBody := hold f
+      let df' := hold fun w i x dx' dw =>
+        let f' : W×X → X := fun (w',x') => f w' i x'
+        let dwx' := gradient K f' (w,x) dx'
+        (dwx'.2, dw + dwx'.1)
+      let xdforIn := ForIn.arg_bf.revDeriv_dataArrayImpl initdinit.1 forInBody df' w
+      (xdforIn.1, 
+       fun dx' => 
+         let (dx'', dw) := xdforIn.2 dx'
+         initdinit.2 dx'' + dw)
+  := sorry_proof
+
+#eval 
+  (⊞ i => gradient Float (fun (x : (Float^Idx 3)×Float) => x.2 * x.1[i]) (⊞[5.0,6,7], 42.0) 1.0)
+    rewrite_by 
+      unfold gradient
+      ftrans
+      simp
+
+
+#check Nat
+
+
+example (i : Idx 3) : HasAdjDiff Float fun (x : Float ^ Idx 3) => x[i] := by fprop
+example (i : Idx 3) : HasAdjDiff Float fun (x : Float ^ Idx 3 × Float) => x.1[i] := by fprop
+
+set_option trace.Meta.Tactic.fprop.step true in
+example (i : Idx (Nat.toUSize 3)) : HasAdjDiff Float fun (x : ((typeOf (5.0 : Float)) ^ Idx (Nat.toUSize 3)) × Float) => x.1[i] := by fprop
+
+set_option pp.funBinderTypes true in
+-- set_option trace.Meta.Tactic.simp.unify true in
+set_option trace.Meta.Tactic.simp.rewrite true in
+set_option trace.Meta.Tactic.simp.discharge true in
+#eval
+  ((gradient Float (fun x : Float ^ Idx 3 => Id.run do
+    let mut y := 1.0
+    for i in fullRange (Idx 3) do
+      y := y * x[i]
+    y))
+    rewrite_by
+      unfold gradient
+      ftrans
+      simp (config:= {zeta:=false}) only [revDerivM]
+      ftrans
+      unfold gradient
+      ftrans
+      ftrans)
+  ⊞[5.0,6,7] 1
+
+-- set_option trace.Meta.Tactic.simp.discharge true in
+-- set_option trace.Meta.Tactic.simp.rewrite true in
+#eval
+  ((gradient Float (fun x : Float ^ Idx 3 => Id.run do
+    let mut y := 1.0
+    for i in fullRange (Idx 3) do
+      let a := y * y
+      y := y * x[i] * a
+    y))
+    rewrite_by
+      unfold gradient
+      ftrans
+      simp (config:= {zeta:=false}) only [revDerivM]
+      ftrans
+      unfold gradient
+      ftrans
+      ftrans)
+  ⊞[5.0,6,7] 1
+
+      
+-- (fun x => Id.run do
+--       let (y₀,dinit') := revCDeriv K init x
+--       let (y,ys) ← forIn (Std.Range.mk start stop step) (y₀,#[]) (fun i (y,ys) => 
+--         let y' := f x i y
+--         .yield (y', ys.push y'))
+--       pure (y, 
+--             fun dy => do
+--               let (dx,dy) ← forIn (Std.Range.mk start stop step) ((0:X),dy) (fun i (dx,dy) => do 
+--                 let j := stop - ((i-start) + 1)
+--                 let yᵢ : Y := ys[j]!
+--                 let (dx',dy) := (revCDeriv K (fun (xy : X×Y) => f xy.1 i xy.2) (x,yᵢ)).2 dy
+--                 .yield (dx + dx', dy))
+--               pure (dx + dinit' dy))) :=
+-- by
+--   sorry_proof
+
+
+
+
+/-- Reverse derivative of `Function.foldl` w.r.t. `f` and `init`. It is implemented using `Array`.
+
+  TODO: 
+    1. needs beter implementation but that requires refining EnumType and Index
+    2. add a version with DataArray
+-/
+def Function.reduceD.revDeriv_dataArrayImpl_alt [PlainDataType X]
+  (f : ι → X) (op : X → X → X) (dop : X → X → X → X×X) (default : X) : X × (X → DataArrayN X ι) := 
+  let n := Index.size ι
+  if n = 0 then
+    (default, fun _ => 0)
+  else Id.run do
+  
+    -- forward pass
+    let mut ys : DataArray X := .mkEmpty n
+    let mut y := f (fromIdx ⟨0,sorry_proof⟩)
+    for i in [1:n.toNat] do 
+      let i : ι := fromIdx ⟨i.toUSize, sorry_proof⟩
+      ys := ys.push y
+      y := op y (f i)
+    (y, 
+     fun dy => Id.run do
+
+       -- backward pass
+       let mut dxs : DataArray X := .mkEmpty n
+       let mut dy := dy
+       for i in [0:n.toNat] do 
+         let j' : Idx n := ⟨n - i.toUSize - 1, sorry_proof⟩
+         let j : ι := fromIdx j'
+         let xj := f j
+         let yj := ys.get ⟨j'.1, sorry_proof⟩
+         let (dy',dx') := dop yj xj dy
+         dxs := dxs.push dx'
+         dy := dy'
+       
+       
+       )
+  -- let bbs := Function.reduceD f (fun (b,bs) a => (op b a, bs.push b)) (default, DataArray.mkEmpty n)
+  -- let b := bbs.1
+  -- let bs := bbs.2
+  -- (b, 
+  --  fun db => Id.run do
+  --    let dbdas := Function.foldl 
+  --      (fun i : Idx n => 
+  --        let j : Idx n := ⟨n-i.1-1, sorry_proof⟩
+  --        (f (fromIdx j), bs.get ⟨j.1, sorry_proof⟩))
+  --      (fun (db,das) (aj,bj) => 
+  --        let (db', da) := dop bj aj db
+  --        (db', das.push da))
+  --      (db, DataArray.mkEmpty n)
+  --    let db := dbdas.1
+  --    let das := dbdas.2
+  --    let das := das.reverse
+  --    (⟨das, sorry_proof⟩, db))
+/--
+TODO: 
+    1. needs beter implementation but that requires refining EnumType and Index
+    2. add a version with DataArray
+-/
+def Function.reduceD.revDeriv_dataArrayImpl_alt [PlainDataType X]
+  (f : ι → X) (op : X → X → X) (dop : X → X → X → X×X) (default : X) : X × (X → DataArrayN X ι) := Id.run do
+  let n := Index.size ι
+  let bbs := Function.reduceD f (fun (b,bs) a => (op b a, bs.push b)) (default, DataArray.mkEmpty n)
+  let b := bbs.1
+  let bs := bbs.2
+  (b, 
+   fun db => Id.run do
+     let dbdas := Function.foldl 
+       (fun i : Idx n => 
+         let j : Idx n := ⟨n-i.1-1, sorry_proof⟩
+         (f (fromIdx j), bs.get ⟨j.1, sorry_proof⟩))
+       (fun (db,das) (aj,bj) => 
+         let (db', da) := dop bj aj db
+         (db', das.push da))
+       (db, DataArray.mkEmpty n)
+     let db := dbdas.1
+     let das := dbdas.2
+     let das := das.reverse
+     (⟨das, sorry_proof⟩, db))
+
+-- /--
+--   TODO: needs beter implementation but that requires refining EnumType and Index
+--   -/
+-- def Function.reduceD (f : ι → α) (op : α → α → α) (default : α) : α := Id.run do
+--   let n := Index.size ι
+--   if n = 0 then
+--     return default
+--   let mut a := f (fromIdx ⟨0,sorry_proof⟩)
+--   for i in [1:n.toNat] do
+--     a := op a (f (fromIdx ⟨i.toUSize,sorry_proof⟩))
+--   return a
+
+
+/-- 
+  TODO: needs beter implementation but that requires refining EnumType and Index
+  -/
+def Function.reduceD.arg_f.revCDeriv [Zero α] 
+  (f df : ι → α) (dop : α → α → α → (α×(α→α×α))) (default : α) : α×α :=   
+  Function.reduceD (fun i => (f i, df i)) (fun (x,dx) (y,dy) => dop x y dx dy) (default, 0)
+
+@[fprop]
+theorem Function.reduceD.arg_fdefault.IsDifferentiable_rule
+  (f : W → ι → X) (op : X → X → X) (default : W → X)
+  (hf : IsDifferentiable K f) (hop : IsDifferentiable K (fun (x,y) => op x y)) (hdefault : IsDifferentiable K default)
+  : IsDifferentiable K (fun w => Function.reduceD (f w) op (default w)) := by sorry_proof
+
+@[ftrans]
+theorem Function.reduceD.arg_fdefault.revCDeriv_rule
+  (f : W → ι → X) (op : X → X → X) (default : W → X)
+  (hf : IsDifferentiable K f) (hop : IsDifferentiable K (fun (x,y) => op x y)) (hdefault : IsDifferentiable K default)
+  : revCDeriv K (fun w => Function.reduceD (f w) op (default w))
+    =
+    fun w dw => 
+      let fdf := revCDeriv K f w dw
+      let defaultddefault := revCDeriv K default w dw
+      let dop := fun (x,dy) (y,dy) => revCDeriv K (fun (x,y) => op x y) (x,y) (dx,dy)
+      Function.reduceD (fun i => (fdf.1 i, fdf.2 i)) dop defaultddefault
+      := by sorry_proof
+
+
+end OnSemiInnerProductSpace
