SciLean/Data/Function.lean
@@ -4,33 +4,36 @@ import SciLean.Data.Index
 def Function.Inverse (g : β → α) (f : α → β) :=
   Function.LeftInverse g f ∧ Function.RightInverse g f
 
-
 open SciLean
 
 variable {α β}
   {ι} [EnumType ι]
 
-def Function.foldl (f : ι → α) (op : β → α → β) (init : β) : β := Id.run do
+def Function.foldlM {m} [Monad m] (f : ι → α) (op : β → α → m β) (init : β) : m β := do
   let mut b := init
   for i in fullRange ι do
-    b := op b (f i)
+    b ← op b (f i)
   return b
 
+def Function.foldl (f : ι → α) (op : β → α → β) (init : β) : β :=
+  Id.run <| Function.foldlM f (fun x y => pure (op x y)) init
 
 variable [Index ι]
 
-/-- 
+/--
   TODO: needs beter implementation but that requires refining EnumType and Index
   -/
-def Function.joinlD (f : ι → α) (op : α → α → α) (default : α) : α := Id.run do
+def Function.reduceMD {m} [Monad m] (f : ι → α) (op : α → α → m α) (default : α) : m α := do
   let n := Index.size ι
   if n = 0 then
     return default
   let mut a := f (fromIdx ⟨0,sorry_proof⟩)
   for i in [1:n.toNat] do
-    a := op a (f (fromIdx ⟨i.toUSize,sorry_proof⟩))
+    a ← op a (f (fromIdx ⟨i.toUSize,sorry_proof⟩))
   return a
 
+def Function.reduceD (f : ι → α) (op : α → α → α) (default : α) : α :=
+  Id.run <| Function.reduceMD f (fun x y => pure (f:=Id) op x y) default
 
-
-
+abbrev Function.reduce [Inhabited α] (f : ι → α) (op : α → α → α) : α := 
+  f.reduceD op default
